The perfect verification module of USKip and USeq completed.

Babel/MetaLanguage/Parity/MetaDuality.v
@@ -22,58 +22,66 @@ Unset Printing Implicit Defensive.
 Section Meta_Duality_Theories.
 
 
-Definition meta_dual (𝑷 : parity) (mT : baseMT 𝑷) 
+Definition meta_dual (mT : baseMT) 
     (f : FType mT -> FType mT) (g : BType mT -> BType mT) : Prop :=
-        forall (P : BType mT) (s : FType mT), (g P) ∙ s ⊑ P ∙ (f s).
+        forall (P : BType mT) (s : FType mT), P ∙ (f s) ⊑ (g P) ∙ s.
 
-Definition bidual (𝑷 : parity) (mT : baseMT 𝑷) 
+
+Definition bidual (mT : baseMT) 
     (f : FType mT -> FType mT) (g : BType mT -> BType mT) : Prop :=
-        meta_dual f g /\ forall (P : BType mT) (s : FType mT), P ∙ (f s) ⊑ (g P) ∙ s.
+        meta_dual f g /\ @meta_dual (Parity_Trans mT) g f.
+
 
 Notation bidual' g := (fun f => bidual f g).
 
 Notation " f ^← " := (ε (bidual f)) : MetaLan_scope.
 Notation " g ^→ " := (ε (bidual' g)) : MetaLan_scope.
 
+
+
 (** IMPORTANT : notice the relation between ' -> ' and the soundness of a
     verification system. *)
-Lemma bwd_correct_dual_sufficiency (mT : bwdMT) 
-    (f : Stt mT -> Stt mT) (g : Asn mT -> Asn mT) :
-        bwd_dual f g -> forall (P Q : Asn_poset mT),  P ⊑ g Q -> ⊨ { P } f { Q }.
+Lemma correct_dual_sufficiency (mT : cpoMT) 
+    (f : FType mT -> FType mT) (g : BType mT -> BType mT) :
+        meta_dual f g -> forall (x y : FType_cpo mT),  
+            x ⊑ f y -> ⊨ { (x : FType mT) } g { y }.
 (** It's necessary to redesign the coercion path! *)
 Proof.
-    move => Hdual P Q.
+    move => Hdual x y.
     move => H.
-        rewrite /bwd_correct => s. 
-        transitivity (g Q ∙ s). by apply Sat_eval_Asn_monotonicity.
+        rewrite /correct => P. 
+        transitivity (P ∙ f y). by apply Sat_eval_monotonicity.
         apply Hdual.
 Qed.
 
-Lemma bwd_correct_dual_necessarity (mT : bwdMT) 
-    (f : Stt mT -> Stt mT) (g : Asn mT -> Asn mT) :
-        fwd_dual g f -> forall (P Q : Asn_poset mT),  ⊨ { P } f { Q } -> P ⊑ g Q.
+
+Lemma correct_dual_necessarity (mT : cpoMT) 
+    (f : FType mT -> FType mT) (g : BType mT -> BType mT) :
+        @meta_dual (Parity_Trans mT) g f -> forall (x y : FType_cpo mT),  
+            ⊨ { (x : FType mT) } g { y } -> x ⊑ f y.
 Proof.
-    move => Hdual P Q.
-    rewrite /bwd_correct => H.
-    apply Sat_eval_Asn_monotonicity => s.
-    transitivity (Q ∙ f s) => //=.
+    move => Hdual x y.
+    rewrite /correct => H.
+    apply Sat_eval_monotonicity => P.
+    transitivity (g P ∙ y). by apply H. by apply Hdual.
 Qed.
 
 (** The existence of backward dual may seems trival in specific cases, but 
     demands a premise in the very general case. *)
-Lemma bwd_correct_duality_expressiveness (mT : bwdMT) (f : Stt mT -> Stt mT):
-    (forall (Q : Asn mT), exists P, ⊨ { P } f { Q }) -> exists g, bwd_dual f g.
+Lemma correct_duality_expressiveness (mT : cpoMT) (g : BType mT -> BType mT):
+    (forall (y : FType mT), exists x, ⊨ { x } g { y }) -> exists f, meta_dual f g.
 Proof.
-    rewrite /bwd_correct => H.
-    exists (fun R => ε (fun P => ∀ s : Stt mT, P ∙ s ⊑ R ∙ f s)).
+    rewrite /correct => H.
+    exists (fun r => ε (fun x => ∀ P : BType mT, P ∙ x ⊑ (g P) ∙ r)).
 
-    rewrite /bwd_dual => Q s.
-    move : (@epsilon_spec _ (λ P : Asn mT, ∀ s0 : Stt mT, P ∙ s0 ⊑ Q ∙ f s0) (H Q)) => //.
+    rewrite /meta_dual => Q s.
+
+    move : (@epsilon_spec _ (λ x : FType mT, ∀ P : BType mT, P ∙ x ⊑ g P ∙ s) (H s)) => //.
 Qed.
 
 
 
-
+(* 
 Lemma lim_bwd_correct (mT : bwdCMT)
     (Ps : 𝒫(Asn mT)) (f : Stt mT -> Stt mT) (Q : Asn mT) :
 
@@ -87,16 +95,29 @@ Proof.
         rewrite Sat_eval_Asn_join_mor => //=. by porder_level.
         by apply H.
 Qed.
+*)
+
+
+
+
+
+
+
+
+
+
+
+    
 
 (** Important *)
-Definition bwd_dual_existence (mT : bwdCMT) (f : Stt mT -> Stt mT) : 
-    { g : Asn mT -> Asn mT | bwd_dual f g }.
+Definition bwd_dual_existence (mT : cLatticeMT) (g : BType mT -> BType mT) : 
+    { f : FType mT -> FType mT | meta_dual f g }.
 Proof.
     econstructor.
     instantiate (1 := 
-        (fun Q => ⊔ᶜˡ ({ P , P | ⊨ { P } f { Q } } : 𝒫(Asn_clattice mT)))).
-    rewrite /bwd_dual => Q s.
-    rewrite Sat_eval_Asn_join_mor => //=.
+        (fun y => ⊔ᶜˡ ({ x , x | ⊨ { x } g { y } } : 𝒫(FType_clattice mT)))).
+    rewrite /meta_dual => Q s.
+    rewrite Sat_eval_join_mor => //=.
     (** QUESTION : is this assumption of join morphism too strong here? *)
 
     apply CLattice.join_prop.
@@ -109,90 +130,68 @@ Qed.
 (** Conclusions about bidual*)
 
 Lemma bidualP (mT : baseMT)
-    (f : Stt mT -> Stt mT) (g : Asn mT -> Asn mT) :
+    (f : FType mT -> FType mT) (g : BType mT -> BType mT):
     bidual f g <-> forall P s, P ∙ f s = g P ∙ s.
 Proof.
-    rewrite /bidual /fwd_dual /bwd_dual. split.
-    - move => [H1 H2] P s. apply poset_antisym. by apply H2. by apply H1.
-    - move => H. split => P s; rewrite H; by reflexivity.
+    rewrite /bidual /meta_dual. split.
+    - move => [H1 H2] P s. apply poset_antisym. by apply H1. by apply H2.
+    - move => H. split => P s. 
+        + rewrite H; by reflexivity.
+        + unfold Parity_Trans in *. simpl in *. rewrite H; by reflexivity.
 Qed.
 
 
-Lemma bidual_unique_bwd (mT : baseMT)
-    (f : Stt mT -> Stt mT)
-    g1 g2 (H1 : bidual f g1) (H2 : bidual f g2) :
-    forall P, g1 P =asn g2 P.
+Lemma bidual_unique (mT : baseMT)
+    (g : BType mT -> BType mT)
+    (f1 f2 : FType mT -> FType mT) (H1 : bidual f1 g) (H2 : bidual f2 g) :
+    forall x, f1 x =FD f2 x.
 Proof.
-    rewrite /sat_asn_eq => P s.
-    rewrite bidualP in H1. rewrite bidualP in H2.
-    by rewrite -H1 -H2.
-Qed.
-
-Lemma bidual_unique_fwd (mT : baseMT)
-    (g : Asn mT -> Asn mT)
-    f1 f2 (H1 : bidual f1 g) (H2 : bidual f2 g) :
-    forall s, f1 s =stt f2 s.
-Proof.
-    rewrite /sat_stt_eq => s P.
+    rewrite /sat_eq => s P.
     rewrite bidualP in H1. rewrite bidualP in H2.
     by rewrite H1 H2.
 Qed.
 
-Lemma bidual_bwd_eq (mT : baseMT)
-    (f : Stt mT -> Stt mT) (g : Asn mT -> Asn mT):
-    bidual f g -> forall P, f ^← P =asn g P.
+
+Lemma bidual_eq (mT : baseMT)
+    (g : BType mT -> BType mT) (f : FType mT -> FType mT):
+    bidual f g -> forall P, g ^→ P =FD f P.
 Proof.
-    move => Hdual. apply (@bidual_unique_bwd _ f).
-    - rewrite /bwd_dual. apply epsilon_PeP. by exists g.
+    move => Hdual. apply (@bidual_unique _ g).
+    - rewrite /meta_dual. apply epsilon_PeP. by exists f.
     - by [].
 Qed.
 
-Lemma bidual_fwd_eq (mT : baseMT)
-    (g : Asn mT -> Asn mT) (f : Stt mT -> Stt mT):
-    bidual' g f -> forall s, g ^→ s =stt f s.
-Proof.
-    move => Hdual. apply (@bidual_unique_fwd _ g).
-    - rewrite /bwd_dual. apply epsilon_PeP. by exists f.
-    - by [].
-Qed.
-
-Lemma bidual_bwd_feq (mT : bwdMT)
-    (f : Stt mT -> Stt mT) (g : Asn mT -> Asn mT):
-        bidual f g -> f ^← = g.
-Proof. 
-    move => Hdual.
-    apply functional_extensionality => P.
-    by apply /bwdMT_sat_eval_Asn_inj /bidual_bwd_eq.
-Qed.
-
-Lemma bidual_fwd_feq (mT : baseMT) (Hinj_Stt : sat_eval_Stt_inj mT)
-    (g : Asn mT -> Asn mT) (f : Stt mT -> Stt mT):
-        bidual' g f -> g ^→ = f.
+Lemma bidual_feq (mT : cpoMT)
+    (g : BType mT -> BType mT) (f : FType mT -> FType mT):
+        bidual f g -> g ^→ = f.
 Proof. 
     move => Hdual.
     apply functional_extensionality => s.
-    by apply /Hinj_Stt /bidual_fwd_eq.
+    by apply /cpoMT_sat_eval_inj /bidual_eq.
 Qed.
 
-Lemma bwd_dual_involutive (mT : baseMT)
-    (Hinj_Stt : sat_eval_Stt_inj mT)
-    (f : Stt mT -> Stt mT):
+Lemma dual_involutive (mT : cpoMT)
+    (Hinj : sat_eval_inj (Parity_Trans mT))
+    (f : FType mT -> FType mT):
     (exists g, bidual f g) -> f ^← ^→ = f.
 Proof.
     move => [g Hg].
-    apply bidual_fwd_feq => //=.
+    apply bidual_feq => //=.
     apply epsilon_PeP.
     by exists g.
 Qed.
 
-Lemma bwd_correct_dual_equiv (mT : bwdMT) 
-    (f : Stt mT -> Stt mT) (g : Asn mT -> Asn mT) :
-        bidual f g -> forall (P Q : Asn_poset mT),  P ⊑ g Q <-> ⊨ { P } f { Q }.
+Lemma correct_dual_equiv (mT : cpoMT) 
+    (f : FType mT -> FType mT) (g : BType mT -> BType mT) :
+        bidual f g -> forall (x y : FType_cpo mT),  
+            x ⊑ f y <-> ⊨ { (x : FType mT) } g { y }.
 Proof.
     move => Hdual P Q. split.
-    - apply /bwd_correct_dual_sufficiency.
+    - apply /correct_dual_sufficiency.
         by apply Hdual.
     
-    - apply /bwd_correct_dual_necessarity.
+    - apply /correct_dual_necessarity.
         by apply Hdual.
 Qed.
+
+End Meta_Duality_Theories.
