Babel/MetaLanguage/Parity/MetaLan.v
@@ -19,32 +19,6 @@ Unset Strict Implicit.
 Unset Printing Implicit Defensive.
 
 
-(****************************************)
-(*                                      *)
-(*       Syntax                         *)
-(*       (Language Syntax)              *)
-(*                                      *)
-(****************************************)
-
-Module Syntax.
-
-Record class : Type := Class {
-    sort : Type;
-}.
-
-Module Exports.
-
-Coercion sort : class >-> Sortclass.
-
-Notation Syn := sort.
-
-Notation syntax := class.
-Notation Syntax s := (Class s).
-
-End Exports.
-
-End Syntax.
-Export Syntax.Exports.
 
 (****************************************)
 (*                                      *)
@@ -55,30 +29,37 @@ Export Syntax.Exports.
 
 
 Module AxSem.
+
 Section ClassDef.
 
-Variable (𝑷 : parity).
-
-Record mixin_of (mT : pTypeMT 𝑷) (Syn : syntax) : Type := Mixin {
-    ax_sys : mT -> Syn -> mT -> Prop;
+Record mixin_of (mT : dMT) (syn : Type) : Type := Mixin {
+    ax_sys : mT -> syn -> mT -> Prop;
 }.
 
-Record class (mT : pTypeMT 𝑷) (syn : syntax): Type := Class {
-    mixin : mixin_of mT syn;
+Notation class_of := mixin_of (only parsing).
+
+Record type (mT : dMT) := Pack {
+    syn : Type;
+    class : class_of mT syn;
 }.
+
 
 End ClassDef.
 
 Module Exports.
 
-Coercion mixin : class >-> mixin_of.
+#[reversible]
+Coercion syn : type >-> Sortclass.
+Coercion class : type >-> mixin_of.
 
-Notation axSem := class.
-Notation AxSem m:= (Class m).
+Notation axSem := type.
+Notation AxSem s m:= (@Pack _ s m).
 
-Notation " ⊢ { P } s { Q } " := (ax_sys (mixin _) P s Q) 
+Notation " ⊢ { P } s { Q } " := (ax_sys _ P s Q) (only printing)
     : MetaLan_scope.
-Notation " ⊢ < ax > { P } s { Q } " := (ax_sys (mixin ax) P s Q) 
+Notation " ⊢ { P } s { Q } " := (ax_sys (class _) P s Q) 
+    : MetaLan_scope.
+Notation " ⊢ < ax > { P } s { Q } " := (ax_sys (class ax) P s Q) 
     : MetaLan_scope.
 
 End Exports.
@@ -86,43 +67,48 @@ End Exports.
 End AxSem.
 Export AxSem.Exports.
 
-(*
+
 
 (****************************************)
 (*                                      *)
-(*       BwdSem                         *)
+(*       DeSem                          *)
 (*       (Backward Transformer)         *)
 (*                                      *)
 (****************************************)
 
 
-Module BwdSem.
+Module DeSem.
 Section ClassDef.
 
-Record mixin_of (mT : bwdMT) (Syn : syntax) : Type := Mixin {
-    wp_fun : Syn -> Asn mT -> Asn mT;
-    wp_monot : forall (s : Syn), MonotonicFun.mixin_of (wp_fun s);
+Record mixin_of (mT : cpo) (syn : Type) : Type := Mixin {
+    de_fun : syn -> mT -> mT;
+    de_monot : forall (s : syn), MonotonicFun.mixin_of (de_fun s);
 }.
 
-Record class (mT : bwdMT) (syn : syntax): Type := Class {
-    mixin : mixin_of mT syn;
+Notation class_of := mixin_of (only parsing).
+
+Record type (mT : cpo) : Type := Pack {
+    syn : Type;
+    class : class_of mT syn;
 }.
 
 End ClassDef.
 
 Module Exports.
 
-Coercion mixin : class >-> mixin_of.
+#[reversible]
+Coercion syn : type >-> Sortclass.
+Coercion class : type >-> mixin_of.
 
-Notation bwdSem := class.
-Notation BwdSem m s := (@Class _ m s).
+Notation deSem := type.
+Notation DeSem s m := (@Pack _ s m).
 
-Notation " 'wp' < bwd > " := (wp_fun bwd) : MetaLan_scope.
+Notation " ⟦ s ⟧ < de > " := (de_fun de s) : MetaLan_scope.
 
 End Exports.
 
-End BwdSem.
-Export BwdSem.Exports.
+End DeSem.
+Export DeSem.Exports.
 
 (****************************************)
 (*                                      *)
@@ -135,32 +121,60 @@ Export BwdSem.Exports.
 Module VeriModS.
 Section ClassDef.
 
-Definition axiom (mT : bwdMT) (syn : syntax)
-    (base_ax : axSem mT syn) (base_bwd : bwdSem mT syn) :=
-        forall (s : Syn syn) (P Q : Asn mT),
-        ⊢ <base_ax> { P } s { Q } -> P ⊑ wp <base_bwd> s P.
+Definition axiom (mT : cpoDMT) (syn : Type)
+    (ax_m : AxSem.mixin_of mT syn) (de_m : DeSem.mixin_of mT syn) 
+    (base_de := DeSem syn de_m) (base_ax := AxSem syn ax_m):=
 
-Record mixin_of (mT : bwdMT) (syn : syntax)
-    (base_ax : axSem mT syn) (base_bwd : bwdSem mT syn) : Type := Mixin {
-    _ : axiom base_ax base_bwd;
+        forall (s : syn) (P Q : [cpo of mT]),
+        ⊢ <base_ax> { P } s { Q } -> P ⊑ ⟦ s ⟧ <base_de> Q.
+
+Record mixin_of (mT : cpoDMT) (syn : Type)
+    (ax_m : AxSem.mixin_of mT syn) (de_m : DeSem.mixin_of mT syn) : Type 
+        := Mixin {
+    soundness : axiom ax_m de_m;
 }.
 
-Record class (mT : bwdMT) (syn : syntax) : Type := Class {
-    base_ax : axSem mT syn;
-    base_bwd : bwdSem mT syn;
-    mixin : mixin_of base_ax base_bwd;
+Record class_of (mT : cpoDMT) (syn : Type) : Type := Class {
+    base_ax : AxSem.mixin_of mT syn;
+    base_de : DeSem.mixin_of mT syn;
+    mixin : mixin_of base_ax base_de;
 }.
+
+Record type (mT : cpoDMT) := Pack {
+    syn : Type;
+    class : class_of mT syn;
+}.
+
+Local Coercion syn : type >-> Sortclass.
+Local Coercion class : type >-> class_of.
+
+Definition to_axSem (mT : cpoDMT) (cT : type mT) :=
+    AxSem (syn cT) (base_ax cT).
+
+Definition to_deSem (mT : cpoDMT) (cT : type mT) :=
+    DeSem (syn cT) (base_de cT).
+
+Definition soundness_of (mT : cpoDMT) (cT : type mT) :=
+    soundness (mixin cT).
+    
 
 End ClassDef.
 
 Module Exports.
 
-Coercion base_ax : class >-> axSem.
-Coercion base_bwd : class >-> bwdSem.
-Coercion mixin : class >-> mixin_of.
+#[reversible]
+Coercion syn : type >-> Sortclass.
+Coercion class : type >-> class_of.
+Coercion mixin : class_of >-> mixin_of.
 
-Notation veriModS := class.
-Notation VeriModS b_ax b_bwd m := (@Class _ _ b_ax b_bwd m).
+Coercion to_axSem : type >-> axSem.
+Coercion to_deSem : type >-> deSem.
+
+Notation veriModS := type.
+Notation VeriModS s m := (@Pack _ s (Class m)).
+
+Arguments soundness_of [_] _.
+Notation soundness_of := soundness_of.
 
 End Exports.
 
@@ -176,39 +190,174 @@ Export VeriModS.Exports.
 (****************************************)
 
 
-(* both sound and complete *)
+(* complete *)
 Module VeriModC.
 Section ClassDef.
 
-Definition axiom (mT : bwdMT) (syn : syntax)
-    (base_ax : axSem mT syn) (base_bwd : bwdSem mT syn) :=
-        forall (s : Syn syn) (P Q : Asn mT),
-        P ⊑ wp <base_bwd> s P -> ⊢ <base_ax> { P } s { Q }.
+Definition axiom (mT : cpoDMT) (syn : Type)
+    (ax_m : AxSem.mixin_of mT syn) (de_m : DeSem.mixin_of mT syn) 
+    (base_ax := AxSem syn ax_m) (base_de := DeSem syn de_m) :=
+        forall (s : syn) (P Q : [cpo of mT]),
+        P ⊑ ⟦ s ⟧ <base_de> Q -> ⊢ <base_ax> { P } s { Q }.
 
 
-Record mixin_of (mT : bwdMT) (syn : syntax)
-    (base_vms : veriModS mT syn) : Type := Mixin {
-    _ : axiom base_vms base_vms;
+Record mixin_of (mT : cpoDMT) (syn : Type)
+    (ax_m : AxSem.mixin_of mT syn) (de_m : DeSem.mixin_of mT syn) 
+        : Type := Mixin {
+    completeness : axiom ax_m de_m;
 }.
 
-Record class (mT : bwdMT) (syn : syntax) : Type := Class {
-    base_vms : veriModS mT syn;
-    mixin : mixin_of base_vms;
+Record class_of (mT : cpoDMT) (syn : Type) : Type := Class {
+    base_ax : AxSem.mixin_of mT syn;
+    base_de : DeSem.mixin_of mT syn;
+    mixin : mixin_of base_ax base_de;
 }.
+
+Record type (mT : cpoDMT) := Pack {
+    syn : Type;
+    class : class_of mT syn;
+}.
+
+Local Coercion syn : type >-> Sortclass.
+Local Coercion class : type >-> class_of.
+
+Definition to_axSem (mT : cpoDMT) (cT : type mT) :=
+    AxSem (syn cT) (base_ax cT).
+
+Definition to_deSem (mT : cpoDMT) (cT : type mT) :=
+    DeSem (syn cT) (base_de cT).
+
+Definition completeness_of (mT : cpoDMT) (cT : type mT) :=
+    completeness (mixin cT).
 
 End ClassDef.
 
 Module Exports.
 
-Coercion base_vms : class >-> veriModS.
-Coercion mixin : class >-> mixin_of.
+#[reversible]
+Coercion syn : type >-> Sortclass.
+Coercion class : type >-> class_of.
+Coercion mixin : class_of >-> mixin_of.
 
-Notation veriModC := class.
-Notation VeriModC b_vms m := (@Class _ _ b_vms m).
+Coercion to_axSem : type >-> axSem.
+Coercion to_deSem : type >-> deSem.
+
+Notation veriModC := type.
+Notation VeriModC s m := (@Pack _ s (Class m)).
+
+Arguments completeness_of [_] _.
+Notation completeness_of := completeness_of.
 
 End Exports.
 
 End VeriModC.
 Export VeriModC.Exports.
 
-*)
+
+    
+(****************************************)
+(*                                      *)
+(*       VeriModSC                      *)
+(*       (Verification Module)          *)
+(*                                      *)
+(****************************************)
+
+
+(* sound and complete *)
+Module VeriModSC.
+Section ClassDef.
+
+Definition axiom (mT : cpoDMT) (syn : Type)
+    (ax_m : AxSem.mixin_of mT syn) (de_m : DeSem.mixin_of mT syn) 
+    (base_ax := AxSem syn ax_m) (base_de := DeSem syn de_m) :=
+        forall (s : syn) (P Q : [cpo of mT]),
+        P ⊑ ⟦ s ⟧ <base_de> Q <-> ⊢ <base_ax> { P } s { Q }.
+
+
+Lemma to_soundness (mT : cpoDMT) (syn : Type)
+    (ax_m : AxSem.mixin_of mT syn) (de_m : DeSem.mixin_of mT syn) 
+    (base_ax := AxSem syn ax_m) (base_de := DeSem syn de_m):
+
+    axiom base_ax base_de -> VeriModS.axiom base_ax base_de.
+Proof. rewrite /axiom /VeriModS.axiom => H s P Q.
+    by rewrite H.
+Qed.
+
+
+Lemma to_completeness (mT : cpoDMT) (syn : Type)
+    (ax_m : AxSem.mixin_of mT syn) (de_m : DeSem.mixin_of mT syn) 
+    (base_ax := AxSem syn ax_m) (base_de := DeSem syn de_m):
+
+    axiom base_ax base_de -> VeriModC.axiom base_ax base_de.
+Proof. rewrite /axiom /VeriModC.axiom => H s P Q.
+    by rewrite H.
+Qed.
+
+
+Record mixin_of (mT : cpoDMT) (syn : Type)
+    (ax_m : AxSem.mixin_of mT syn) (de_m : DeSem.mixin_of mT syn)
+    (veriS_m : VeriModS.mixin_of ax_m de_m) 
+    (veriC_m : VeriModC.mixin_of ax_m de_m) 
+        : Type := Mixin {
+}.
+
+
+Lemma combine (mT : cpoDMT) (syn : Type)
+    (ax_m : AxSem.mixin_of mT syn) (de_m : DeSem.mixin_of mT syn) 
+    (veriS_m : VeriModS.mixin_of ax_m de_m) 
+    (veriC_m : VeriModC.mixin_of ax_m de_m) :
+
+    axiom ax_m de_m.
+
+Proof. rewrite /axiom => s P Q. split.
+    destruct veriC_m as [H_C]. by apply H_C. 
+    destruct veriS_m as [H_S]. by apply H_S.
+Qed.
+
+
+Record class_of (mT : cpoDMT) (syn : Type) : Type := Class {
+    base_ax : AxSem.mixin_of mT syn;
+    base_de : DeSem.mixin_of mT syn;
+    equiv : axiom base_ax base_de;
+}.
+
+Record type (mT : cpoDMT) := Pack {
+    syn : Type;
+    class : class_of mT syn;
+}.
+
+Local Coercion syn : type >-> Sortclass.
+Local Coercion class : type >-> class_of.
+
+Definition pack (mT : cpoDMT) (syn : Type) 
+    (ax_m : AxSem.mixin_of mT syn) (de_m : DeSem.mixin_of mT syn)
+    (veriS_m : VeriModS.mixin_of ax_m de_m) 
+    (veriC_m : VeriModC.mixin_of ax_m de_m) 
+    (m : mixin_of veriS_m veriC_m) : type mT :=
+        Pack (Class (combine veriS_m veriC_m)).
+
+Definition to_veriModS (mT : cpoDMT) (cT : type mT) :=
+    VeriModS (syn cT) (VeriModS.Mixin (to_soundness (equiv cT))).
+
+Definition to_veriModC (mT : cpoDMT) (cT : type mT) :=
+    VeriModC (syn cT) (VeriModC.Mixin (to_completeness (equiv cT))).
+
+End ClassDef.
+
+Module Exports.
+
+#[reversible]
+Coercion syn : type >-> Sortclass.
+Coercion class : type >-> class_of.
+
+Coercion to_veriModS : type >-> veriModS.
+Coercion to_veriModC : type >-> veriModC.
+
+Notation veriModSC := type.
+Notation VeriModSC s m := (@pack _ s _ _ _ _ m).
+
+End Exports.
+
+End VeriModSC.
+Export VeriModSC.Exports.
+
