Babel/MetaLanguage/UFeatures/USeq.v
@@ -1,0 +1,127 @@
+(** USeq.v *)
+From Babel Require Import TerminalDogma 
+                          ExtraDogma.Extensionality
+                          EpsilonDescription
+                          SetFacility
+                          POrderFacility.
+
+From Babel Require Import Ranko
+                            ExtensionalityCharacter
+                            ClassicalCharacter.
+
+From Babel.MetaLanguage Require Import Notations
+                                        MetaType
+                                        MetaLan.
+
+From Coq Require Import Relations Classical.
+
+Set Implicit Arguments.
+Unset Strict Implicit.
+Unset Printing Implicit Defensive.
+
+(** Do not import this module. *)
+Module USeq.
+
+
+(** Syntax *)
+
+Record syn (syn0 syn1 : Type) := seq_ {
+    S0 : syn0;
+    S1 : syn1;
+}.
+
+Notation "s0 ⨾ s1" := {| S0 := s0; S1 := s1 |} : MetaLan_scope.
+
+
+(** DeSem 
+    For now let's consider backward semantics.
+*)
+
+Definition de_fun (mT : cpo) (de0 de1 : deSem mT): syn de0 de1 -> mT -> mT := 
+    fun s P => ⟦ S0 s ⟧ <de0> (⟦ S1 s ⟧ <de1> P).
+
+Lemma de_fun_monot (mT : cpo) (de0 de1 : deSem mT): 
+    forall s, MonotonicFun.mixin_of (@de_fun mT de0 de1 s).
+Proof. 
+    porder_level.
+    rewrite /de_fun.
+    apply DeSem.de_monot.
+    by apply DeSem.de_monot. 
+Qed.
+
+Definition deSem_mixin (mT : cpo) (de0 de1 : deSem mT) : 
+    DeSem.mixin_of mT (syn de0 de1) :=
+{|
+	DeSem.de_fun := @de_fun mT de0 de1;
+    DeSem.de_monot := @de_fun_monot mT de0 de1;
+|}.
+
+Definition deSem (mT : cpo) (de0 de1 : deSem mT) := 
+    DeSem (syn de0 de1) (deSem_mixin de0 de1).
+
+
+
+(** AxSem *)
+
+Inductive ax_sys (mT : dMT) (ax0 ax1 : axSem mT) : 
+    mT -> syn ax0 ax1 -> mT -> Prop :=
+
+| RULE_SEQ 
+        (s0 : ax0) (s1 : ax1) (P R Q : mT) 
+        (H0 : ⊢ { P } s0 { R }) 
+        (H1 : ⊢ { R } s1 { Q }): ax_sys P (s0 ⨾ s1)  Q.
+
+Definition axSem_mixin (mT : dMT) (ax0 ax1 : axSem mT) : 
+        AxSem.mixin_of mT (syn ax0 ax1)
+    := AxSem.Mixin (@ax_sys _ ax0 ax1).
+
+Definition axSem (mT : dMT) (ax0 ax1 : axSem mT) := 
+    AxSem (syn ax0 ax1) (axSem_mixin ax0 ax1).
+
+
+(** VeriModS *)
+
+Definition veriModS_mixin (mT : cpoDMT) (veriS0 veriS1 : veriModS mT): 
+    VeriModS.mixin_of (axSem veriS0 veriS1) (deSem veriS0 veriS1).
+Proof. 
+    constructor. rewrite /VeriModS.axiom => [] [] s0 s1 P Q.
+    move => [] //=. intros. rewrite /de_fun.
+    apply (soundness_of veriS1) in H1 => //=.
+    apply (soundness_of veriS0) in H0 => //=.
+    
+    transitivity ((⟦ s2 ⟧ < DeSem veriS0 (VeriModS.base_de veriS0) >) R).
+    - by [].
+    - by apply (DeSem.de_monot).
+Qed.
+
+Definition veriModS (mT : cpoDMT) (veriS0 veriS1 : veriModS mT) := 
+    VeriModS (syn veriS0 veriS1) (veriModS_mixin veriS0 veriS1).
+
+(** VeriModC *)
+
+
+Definition veriModC_mixin (mT : cpoDMT) (veriC0 veriC1 : veriModC mT): 
+    VeriModC.mixin_of (axSem veriC0 veriC1) (deSem veriC0 veriC1).
+Proof. 
+    constructor. rewrite /VeriModC.axiom => [] [] s0 s1 P Q. simpl.
+    rewrite /de_fun => //= H.
+    eapply RULE_SEQ.
+    instantiate (1 := (⟦ s1 ⟧ < VeriModC.base_de veriC1 >) Q).
+
+    by apply (completeness_of _).
+    apply (completeness_of _); by reflexivity.
+Qed.
+
+Definition veriModC (mT : cpoDMT) (veriC0 veriC1 : veriModC mT) := 
+    VeriModC (syn veriC0 veriC1) (veriModC_mixin veriC0 veriC1).
+
+(** VeriModSC *)
+
+Definition veriModSC_mixin (mT : cpoDMT) (veri0 veri1 : veriModSC mT) : 
+    VeriModSC.mixin_of (veriModS veri0 veri1) (veriModC veri0 veri1).
+Proof. constructor. Qed.
+
+Definition veriModSC (mT : cpoDMT) (veri0 veri1 : veriModSC mT) := 
+    VeriModSC (syn veri0 veri1) (veriModSC_mixin veri0 veri1).
+
+End USeq.
