Babel/MetaLanguage/Notations.v
@@ -4,7 +4,10 @@ Declare Scope MetaLan_scope.
 Open Scope MetaLan_scope.
 
 Reserved Notation " P ∙ s " (at level 20).
+Reserved Notation " P ∙ s :> mT" (at level 20, s at next level).
 Reserved Notation " ⌈ P ⇒ Q ⌉ ".
+Reserved Notation " ⌈ P ⇒ Q ⌉ :> mT " (at level 20, Q at next level).
+
 Reserved Notation " P '=FD' Q " (at level 70).
 Reserved Notation " x '=BD' y " (at level 70).
 
@@ -13,12 +16,17 @@ Reserved Notation " ⊨ { P } f { Q } " (at level 10, P, f, Q at next level).
 Reserved Notation " ⊨ [ x ] g [ y ] " (at level 10, x, g, y at next level).
 
 (** Note that the following two only talks in the syntax level. *)
+Reserved Notation " ax ⊢ P ⇒ Q " (at level 10, P, Q at next level).
+
+
 Reserved Notation " ⊢ { P } s { Q } " (at level 10, P, s, Q at next level).
 Reserved Notation " ⊢ < ax > { P } s { Q } " (at level 10, ax, P, s, Q at next level).
 Reserved Notation " ⊢ [ x ] s [ y ] " (at level 10, x, s, y at next level).
 
-Reserved Notation " 'wp' < bwd > " (at level 50, bwd at next level).
+Reserved Notation " ⟦ s ⟧ < de > " (at level 50, de at next level).
 
 
 Reserved Notation " f ^← " (at level 90). 
 Reserved Notation " g ^→ " (at level 90).
+
+Reserved Notation "s0 ⨾ s1" (at level 50).
